Hierarchy of levels basically working

theories/embeddingUniverses.v
@@ -6,16 +6,15 @@ Require Import FunctionalExtensionality.
 Require Import Coq.Logic.PropExtensionality.
 
 Definition nil := <Nil>.
-Definition cons := <fun env => fun ty => cons env ty>.
+Definition cons := <fun ctx => fun lvl => fun ty => Cons ctx lvl ty>.
 
 Definition zero := <fun env => proj2 env>.
 Definition succ := <fun x => fun env => x (proj1 env)>.
 
-Definition lzero := <lzero>.
-Definition lsuc := <lsuc>.
+Definition level (n : nat) : QTerm := const n.
 (* Should I have an explicit type level on the pis? *)
 Definition pi := <fun x => fun y => fun env => Pi (x env) (fun a => y (env , a))>.
-Definition U : QTerm := <fun lvl => fun env => U lvl>.
+Definition U : QTerm := <(*fun lvl => *)fun env => U (*lvl*)>.
 Definition Empty := <fun env => Empty>.
 Definition Bool := <fun env => Bool>.
 Definition Lift := <fun T => fun env => Lift T>.
@@ -31,93 +30,93 @@ Definition weaken := <fun t => fun env => t (proj1 env)>.
 Definition subLast := <fun t => fun toSub => fun env => t (env , toSub env)>.
 
 Ltac unfold_all := unfold nil, cons, zero, succ, pi, U, Bool, Empty, var_to_term, lambda,
-    app, weaken, subLast, lzero, lsuc, true, false, ifexpr in *.
+    app, weaken, subLast, level, true, false, ifexpr in *.
 
 (* The deeper shallow embedding *)
 
-Inductive VarTyped : QTerm -> QTerm -> QTerm -> Prop :=
-| ty_zero : forall ctx T, VarTyped <`cons `ctx `T> <`weaken `T> zero
-| ty_succ : forall ctx A T s, VarTyped ctx A s
-                              -> VarTyped <`cons `ctx `T> <`weaken `A> <`succ `s>.
+Inductive VarTyped : QTerm -> nat -> QTerm -> QTerm -> Prop :=
+| ty_zero : forall ctx T lvl, VarTyped <`cons `ctx {const lvl} `T> lvl <`weaken `T> zero
+| ty_succ : forall ctx A T s lvl1 lvl2, VarTyped ctx lvl1 A s
+                              -> VarTyped <`cons `ctx `lvl2 `T> lvl1 <`weaken `A> <`succ `s>.
 
-Inductive Typed : QTerm -> QTerm -> QTerm -> Prop :=
+Inductive Typed : (*context*) QTerm -> (*level*) nat -> (*Type*) QTerm -> (*Term*) QTerm -> Prop :=
 | ty_lambda : forall ctx A B s lvl,
-    Typed ctx <`U `lvl> <`pi `A `B> ->
-    Typed <`cons `ctx `A> B s -> Typed ctx <`pi `A `B> <`lambda `s>
-| ty_app : forall ctx A B s1 s2, Typed ctx <`pi `A `B> s1 -> Typed ctx A s2
-                                 -> Typed ctx <`subLast `B `s2> <`app `s1 `s2>
-| ty_var : forall ctx T t, VarTyped ctx T t -> Typed ctx T t
-| ty_true : forall ctx, Typed ctx Bool true
-| ty_false : forall ctx, Typed ctx Bool false
-| ty_if : forall ctx T cond t1 t2,
-    Typed ctx Bool cond ->
-    Typed ctx <`subLast `T `true> t1 ->
-    Typed ctx <`subLast `T `false> t2 ->
-    Typed ctx <`subLast `T `cond> <`ifexpr `cond `t1 `t2>
-| ty_Empty : forall ctx, Typed ctx <`U `lzero> Empty
-| ty_Bool : forall ctx, Typed ctx <`U `lzero> Bool
+    Typed ctx (S lvl) <`U(*{const lvl}*)> <`pi `A `B> ->
+    Typed <`cons `ctx {const lvl} `A> lvl B s -> Typed ctx lvl <`pi `A `B> <`lambda `s>
+| ty_app : forall ctx A B s1 s2 lvl, Typed ctx lvl <`pi `A `B> s1 -> Typed ctx lvl A s2
+                                 -> Typed ctx lvl <`subLast `B `s2> <`app `s1 `s2>
+| ty_var : forall ctx T t lvl, VarTyped ctx lvl T t -> Typed ctx lvl T t
+| ty_true : forall ctx, Typed ctx 0 Bool true
+| ty_false : forall ctx, Typed ctx 0 Bool false
+| ty_if : forall ctx T cond t1 t2 lvl,
+    Typed ctx lvl Bool cond ->
+    Typed ctx lvl <`subLast `T `true> t1 ->
+    Typed ctx lvl <`subLast `T `false> t2 ->
+    Typed ctx lvl <`subLast `T `cond> <`ifexpr `cond `t1 `t2>
+| ty_Empty : forall ctx, Typed ctx 1 <`U(*{const 0}*)> Empty
+| ty_Bool : forall ctx, Typed ctx 1 <`U(*{const 0}*)> Bool
 | ty_pi : forall ctx A B lvl,
-    Typed ctx <`U `lvl> A
-    -> Typed <`cons `ctx `A> <`U `lvl> B -> Typed ctx <`U `lvl> <`pi `A `B>
-| ty_U : forall ctx lvl,
-    Typed ctx <`U (`lsuc `lvl)> <`U lvl>
-.
+    Typed ctx (S lvl) <`U(*{const lvl}*)> A
+    (* TODO: is S lvl correct below? *)
+    -> Typed <`cons `ctx {const lvl} `A> (S lvl) <`U(*{const lvl}*)> B -> Typed ctx (S lvl) <`U(*{const lvl}*)> <`pi `A `B>
+| ty_U : forall ctx lvl, Typed ctx (S (S lvl)) <`U(*{const (S lvl)}*)> <`U(*{const lvl}*)>.
 
 Ltac solve_no_unfold := repeat (lambda_solve ; repeat neutral_inj_case ;lambda_solve
                   ; repeat fast_neutral_unequal_case). 
 
 Ltac solve_all := repeat (unfold_all ; lambda_solve ; repeat neutral_inj_case ;lambda_solve
-                  ; repeat fast_neutral_unequal_case). 
+                          ; repeat fast_neutral_unequal_case).
 
-Inductive In': QTerm -> (QTerm -> Prop) -> Prop:=
-| in_Pi : forall (S : QTerm -> Prop) (F : QTerm -> (QTerm -> Prop)) A B,
-    In' A S
-    -> (forall a, S a -> In' <`B `a> (F a))
-    -> In' <Pi `A `B> (fun f => forall a (s : S a), F a <`f `a>)
-| in_Bool :  In' <Bool> (fun b => b = <fun x => proj1 x> \/ b = <fun x => proj2 x>)
-| in_Empty : In' <Empty> (fun _ => False).
+Inductive In' (I : QTerm -> Prop) : QTerm -> (QTerm -> Prop) -> Prop:=
+| in_Pi : forall (s : QTerm -> Prop) (F : QTerm -> (QTerm -> Prop)) A B,
+    In' I A s
+    -> (forall a, s a -> In' I <`B `a> (F a))
+    -> In' I <Pi `A `B> (fun f => forall a (s : s a), F a <`f `a>)
+| in_Bool :  In' I <Bool> (fun b => b = <fun x => proj1 x> \/ b = <fun x => proj2 x>)
+| in_Empty : In' I <Empty> (fun _ => False)
+(* TODO: Put lvl in type? or get rid of them? *)
+| in_type : In' I <U> I.
 
-Inductive In : QTerm -> (QTerm -> Prop) -> Prop :=
-| in' : forall T S, In' T S -> In T S
-| in_type : In <U> (fun T => exists S, In' T S).
+(* In (S n) represents the interperetation of a type at level n *)
+Fixpoint In (lvl : nat) : QTerm -> (QTerm -> Prop) -> Prop :=
+  match lvl with
+  | O => fun _ _ => False (* TODO: Is this how I want to do it? *)
+  | S lvl' => In' (fun T => exists S, In lvl' T S)
+  end.
 
-Theorem In_function : forall T S1 S2, In T S1 -> In T S2 -> S1 = S2.
-Proof with (try (intros; inversion H; inversion H0; solve_all; reflexivity; fail)).
-  intros T S1 S2 in1.
+Theorem In_function : forall lvl T S1 S2, In lvl T S1 -> In lvl T S2 -> S1 = S2.
+Proof.
+  intros lvl T S1 S2 in1.
   generalize dependent S2.
-  destruct in1 as [T S in1 | typeCase].
-  - induction in1 as [ S F A B In_A_S In_A_S_only In_Ba_Fa In_Ba_Fa_only | | ]...
+  destruct lvl.
+  - inversion in1.
+  -
+    (* All cases other than Pi X Pi can be dealt with trivially*)
+    induction in1; try(intros; inversion H; solve_all; fail).
     intros S2 in2.
-    inversion in2 as [T S'' in2' | ]; solve_all.
-    inversion in2' as [S' F' A' B' In_A_S' In_Ba_F'a eq extra | | ]; solve_all.
-    solve_all.
-    rewrite (In_A_S_only S' (in' _ _ In_A_S')) in *.
+    inversion in2; solve_all.
     subst.
+    rewrite <- (IHin1 s0 H2) in *.
     extensionality f.
     extensionality a.
     extensionality Sa.
-    rewrite (In_Ba_Fa_only a Sa (F' a) (in' _ _ (In_Ba_F'a a Sa))).
+    rewrite (H0 a Sa (F0 a) (H3 a Sa)).
     reflexivity.
-  - intros.
-    inversion H.
-    inversion H0; solve_all. (* Type x anything cases*)
-    reflexivity. (* Type Type case*)
 Qed.
 
 Inductive InCtx : QTerm -> QTerm -> Prop :=
 | in_nil : InCtx nil nil
-| in_cons : forall env ctx val T S,
+| in_cons : forall env ctx lvl val T s,
     InCtx env ctx
-    -> In <`T `env> S
-    -> S val
-    -> InCtx <`env , `val> <`cons `ctx `T>.
+    -> In (S lvl) <`T `env> s (* is the successor here correct? *)
+    -> s val
+    -> InCtx <`env , `val> <`cons `ctx {const lvl} `T>.
 
-
-Theorem fundamental_lemma : forall ctx T t env,
-    Typed ctx T t
+Theorem fundamental_lemma : forall ctx T lvl t env,
+    Typed ctx lvl T t
     -> InCtx env ctx
-    -> exists S, In <`T `env> S
-    /\ S <`t `env>.
+    -> exists s, In (S lvl) <`T `env> s (* TODO: S lvl? In 0 is just empty. *)
+    /\ s <`t `env>.
 Proof.
   intros.
   generalize dependent env.
@@ -125,39 +124,40 @@ Proof.
   (* lambda *)
   - intros env inctx.
     specialize (IHTyped1 env inctx) as [SU [InU piAB_in_SU]].
-    inversion InU; clear InU; subst; [inversion H1|]; solve_all.
+    inversion InU; clear InU; solve_all.
+    (*inversion InU; clear InU; subst; [inversion H1|]; solve_all.*)
+    subst.
     destruct piAB_in_SU as [SPiAB In'PiAB].
     inversion In'PiAB; clear In'PiAB; solve_all.
-    exists (fun f : QTerm => forall a : QTerm, S a -> F a <`f `a>).
+    exists (fun f : QTerm => forall a : QTerm, s0 a -> F a <`f `a>).
     split.
     + repeat constructor; intros; eauto.
     + intros a SAa.
       specialize (H3 a SAa).
       solve_all.
       specialize (IHTyped2 <`env , `a>).
-      replace <cons `ctx `A> with <`cons `ctx `A> in IHTyped2 by (unfold cons; normalize; reflexivity).
-      destruct (IHTyped2 (in_cons _ _ _ _ S inctx (in' _ _ H2) SAa)) as [Fa' [InBFa' Fa's]].
-      rewrite (In_function _ _ _ (in' _ _ H3) InBFa').
+      replace <Cons `ctx {const lvl} `A> with <`cons `ctx {const lvl} `A> in IHTyped2 by (unfold cons; normalize; reflexivity).
+      Check (in_cons _ _ _ _ _ s0 inctx H2).
+      destruct (IHTyped2 (in_cons _ _ _ _ _ s0 inctx H2 SAa)) as [Fa' [InBFa' Fa's]].
+      rewrite (In_function (S _) _ _ _ H3 InBFa').
       apply Fa's.
   (* app *)
   - intros env inctx.
     specialize (IHTyped1 env inctx) as [SPIAB [inPiAB s1Elem]].
     specialize (IHTyped2 env inctx) as [SA [inA s2Elem]].
-    inversion inPiAB as [T S in'PiAB |]; solve_all.
-    inversion in'PiAB as [ SA' F A' B' In_A'_SA' In_B'a_F'a eq | |]; solve_all; subst.
-    replace SA' with SA in * by (symmetry; apply (In_function _ _ _ (in' _ _ In_A'_SA') inA)).
+    inversion inPiAB as [SA' F A' B' In_A'_SA' In_B'a_F'a eq | | | ]; solve_all.
+    subst.
+    (*inversion in'PiAB as [ SA' F A' B' In_A'_SA' In_B'a_F'a eq | |]; solve_all; subst.*)
+    replace SA' with SA in * by (symmetry; apply (In_function (S _) _ _ _ In_A'_SA' inA)).
     exists (F <`s2 `env>).
     specialize (In_B'a_F'a <`s2 `env> s2Elem).
     specialize (s1Elem <`s2 `env> s2Elem).
     normalize_in In_B'a_F'a.
-    split.
-    + apply in'.
-      apply In_B'a_F'a.
-    + apply s1Elem.
+    split; auto.
   (* var *)
   - intros env inctx.
     generalize dependent env.
-    induction H; intros x inctx; inversion inctx; solve_all; eauto.
+    induction H; intros x inctx; inversion inctx; solve_all; subst; eauto.
   (* true *)
   - intros env inctx.
     eexists.
@@ -171,8 +171,7 @@ Proof.
   (* if *)
   - intros env inctx.
     specialize (IHTyped1 env inctx) as [S [In_Bool_S S_cond]].
-    inversion In_Bool_S as [T0 S0' In_Bool_S' | ]; solve_all.
-    inversion In_Bool_S'; solve_all.
+    inversion In_Bool_S; solve_all.
     subst.
     destruct S_cond.
     + (*true*)
@@ -218,19 +217,23 @@ Proof.
     normalize.
     split; [apply in_type|].
     specialize (IHTyped1 env inctx) as [SAU [InUSA SAA]].
-    inversion InUSA. {inversion H1; solve_all.}
+    inversion InUSA; try solve [solve_all].
     subst.
     destruct SAA as [SA InASA].
     unfold pi.
     normalize.
     eexists.
-    pose (fun (a b : QTerm) => exists SB, In' <`B (`env , `a)> SB /\ SB b) as F.
+    pose (fun (a b : QTerm) => exists SB, In (S lvl) <`B (`env , `a)> SB /\ SB b) as F.
     apply in_Pi with (F := F); eauto.
 
     intros.
-    specialize (IHTyped2 <`env, `a> (in_cons _ _ _ _ _ inctx (in' _ _ InASA) H1)) as [SU [InUS BinSU]].
+    Check in_cons.
+    Check (in_cons _ _ _ _ _ _ inctx InASA H1).
+    Check a.
+
+    specialize (IHTyped2 <`env, `a> (in_cons _ _ _ _ _ _ inctx InASA H1)) as [SU [InUS BinSU]].
     solve_all.
-    rewrite <- (In_function _ _ _ InUSA InUS) in BinSU.
+    rewrite <- (In_function (S (S _)) _ _ _ InUSA InUS) in BinSU.
     destruct BinSU as [SB In'BSB].
 
     replace SB with ((fun _ => SB) a) in In'BSB by reflexivity.
@@ -241,14 +244,26 @@ Proof.
     split; intros; eauto.
     destruct H2.
     destruct H2.
-    rewrite (In_function _ _ _ (in' _ _ In'BSB) (in' _ _ H2)).
+    rewrite (In_function (S _) _ _ _ In'BSB H2).
     auto.
+  (* Type n : Type (S n) *)
+  - intros.
+    eexists.
+    split.
+    + unfold U.
+      normalize.
+      apply in_type.
+    + simpl.
+      eexists.
+      unfold U.
+      normalize.
+      apply in_type.
 Qed.
      
-Theorem consistency : forall t, Typed nil Empty t -> False.
+Theorem consistency : forall t, Typed nil 0 Empty t -> False.
 Proof.
   intros.
-  destruct (fundamental_lemma nil Empty t nil H in_nil) as [S [InEmptyS H1]].
+  destruct (fundamental_lemma nil Empty 0 t nil H in_nil) as [S [InEmptyS H1]].
   inversion InEmptyS; inversion H0; solve_all.
   subst.
   auto.
